WeirdLogic/Example4.lean
@@ -158,13 +158,13 @@ def lang_squeeze_list: Set trm :=
 def lang_fun_set : Set trm :=
   {[lang| fun ⸨xl: Loc⸩ ⸨yl : Loc⸩ => {tt}] | tt ∈ lang_squeeze_list' }
 -/
-def pay_index : Set (trm × Example3.payload × payload) :=
+def pay_index : Set (trm × payload × payload) :=
   { x |
-    ∃ p1 ∈ @Set.univ Example3.payload, ∃ p2 ∈ @Set.univ payload, (default_trm,(p1,p2))=x
+    ∃ p1 ∈ @Set.univ payload, ∃ p2 ∈ @Set.univ payload, (default_trm,(p1,p2))=x
   }
 
-def lang_index : Set (trm × Example3.payload × payload ):=
-  { (l, (Example3.default_payload,default_payload)) | l ∈ lang_squeeze_list'}
+def lang_index : Set (trm × payload × payload ):=
+  { (l, (default_payload,default_payload)) | l ∈ lang_squeeze_list'}
 /-
 def lang_index1 : Set (trm × payload × payload ):=
   { (l, (default_payload,default_payload)) | l  ∈ {trm_seq (cfgexp_grammar i trm1 trm2) (trm3) | i : ℕ } }
@@ -261,13 +261,61 @@ lemma example4_spec (xv : ℤ) (yv : ℤ):
   {
     [∗ in ⟪0,pay_index⟫ ∪ ⟪1,lang_index⟫ | xl ~~> xv ∗ yl ~~> yv]
   }
-  [0| p in pay_index => prog_c1(⸨xl : Loc⸩, ⸨yl : Loc⸩, ⟨Int.ofNat p.val.2.1⟩, ⟨p.val.2.2⟩) ]
+  [0| p in pay_index => prog_c1(⸨xl : Loc⸩, ⸨yl : Loc⸩, ⟨p.val.2.1⟩, ⟨p.val.2.2⟩) ]
   [1| l in lang_index => ⌜ tfunc l.val.fst ⌝(⸨xl: Loc⸩, ⸨yl : Loc⸩)]
   { v,
     fun h => ∀ ll ∈ lang_index, ∃ pp ∈ pay_index , h ⟨1, ll⟩ = h ⟨0, pp⟩
   }
   := by
   intro tfunc
+
+  let s' := { (default_trm, p, p2) | (p : ℤ) (p2 : ℤ) (_h : 0 ≤ p) }
+  rw [← bighstar_hhstar_disj_dir
+    (s₁ := ⟪0, pay_index⟫ \ ⟪0, s'⟫)
+    (s₂ := ⟪0, s'⟫ ∪ ⟪1, lang_index⟫)]
+  on_goal 2=>
+    simp [disjoint_label_set, pay_index, s']
+    rw [Set.disjoint_iff_forall_ne]
+    aesop
+  on_goal 2=>
+    ext a ; rcases a with ⟨_, ⟨_, _, _⟩⟩ ; simp [s', pay_index] ; aesop ; omega
+
+  apply weird_weaken_lemma (s' := s')
+  { simp }
+  { simp }
+  { simp [s', pay_index] ; aesop }
+  { simp [disjoint_label_set] }
+  { simp }
+  { simp
+    have tmp := htriple_prod (α := (trm × payload × payload)ˡ)
+      (s := ⟪0, pay_index \ s'⟫)
+      (ht := fun p ↦ prog_c1.trm_call [xl, yl, [lang| ⟨p.val.2.1⟩], [lang| ⟨p.val.2.2⟩]])
+      (H := fun _ => xl ~~> xv ∗ yl ~~> yv)
+      (Q := fun _ _ => htop)
+    specialize tmp ?_
+    { clear tmp
+      rintro ⟨_, ⟨_, _, _⟩⟩ ha ; simp [pay_index, s'] at ha ; rcases ha with ⟨_, _, ha⟩ ; subst_eqs ; simp at ha
+      unfold prog_c1 ; dsimp
+      xwp; xseq_xlet_if_needed
+      unfold Example3.prog_c1
+      xwp; xseq_xlet_if_needed
+      apply xfor_empty_lemma ; omega
+      xsimp
+      apply xfor_empty_lemma ; omega
+      xsimp
+      unfold Example0.prog_c1
+      xstep ; xstep ; xwp ; xapp triple_gt
+      rename_i snd rr ; cases (decide (snd > 10)) <;> xwp <;> xif <;> intros <;> try contradiction
+      · xstep ; xapp ; xsimp
+      · xstep ; xapp ; xsimp
+    }
+    unfold LGTM.wp ; simp ; rw [hwp_ht_eq] ; apply htriple_conseq ; apply tmp
+    · ysimp
+    · ysimp
+    · whnf ; aesop
+  }
+  simp [s']
+
   yin 1 :
     try (first
       | (apply ywp_lemma_funs;
@@ -301,11 +349,11 @@ lemma example4_spec (xv : ℤ) (yv : ℤ):
   apply LGTM.triple_conseq-- ; apply hhimpl_refl ; rotate_left
   rotate_left ; rotate_left
   apply weird_gram_seq_full_prod
-    (α := (trm × Example3.payload × payload)ˡ)
-    (β := (trm × Example3.payload)ˡ)
+    (α := (trm × payload × payload)ˡ)
+    (β := (trm × payload)ˡ)
     (γ := (trm × payload)ˡ)
     (sht_prog1 := LGTM.SHT.mk ⟪0, Example3.pay_index⟫
-      fun p ↦ Example3.prog_c1.trm_call [xl, yl, [lang| ⟨Int.ofNat p.val.2⟩]])
+      fun p ↦ Example3.prog_c1.trm_call [xl, yl, [lang| ⟨p.val.2⟩]])
     (sht_lang1 := LGTM.SHT.mk ⟪1, Example3.lang_index⟫
       fun l ↦ l.val.1.trm_call [xl, yl])
     (sht_prog2 := LGTM.SHT.mk ⟪0, Example0.pay_index⟫
@@ -320,12 +368,12 @@ lemma example4_spec (xv : ℤ) (yv : ℤ):
       hforall fun j =>
       hforall fun (_ :
       n ∈ (({⟨0, (default_trm, j)⟩} ∪
-      {⟨1, ([lang| fun ⸨xl: Loc⸩ ⸨yl : Loc⸩=> {Example3.cfgexp_grammar j Example3.trm1 Example3.trm2}], Example3.default_payload)⟩}) : Set (trm × Example3.payload)ˡ)) =>
+      {⟨1, ([lang| fun ⸨xl: Loc⸩ ⸨yl : Loc⸩=> {Example3.cfgexp_grammar j Example3.trm1 Example3.trm2}], default_payload)⟩}) : Set (trm × payload)ˡ)) =>
       (xl ~~> (xv + Int.ofNat j) ∗ yl ~~> (yv + Int.ofNat j)))
   { simp [lang_index, lang_squeeze_list']
-    exists (((lang_part1 0).trm_seq (lang_part2 false)), Example3.default_payload, default_payload)
+    exists (((lang_part1 0).trm_seq (lang_part2 false)), default_payload, default_payload)
     simp }
-  { simp [pay_index] ; exists (default_trm, Nat.zero, 0) ; simp }
+  { simp [pay_index] ; exists (default_trm, 0, 0) ; simp }
   { clear aux haux
     ext a ; dsimp only ; rcases a with ⟨⟨al, ⟨atrm, ap⟩⟩, ⟨bl, ⟨btrm, bp⟩⟩⟩
     simp [lang_index, lang_squeeze_list',
@@ -353,9 +401,9 @@ lemma example4_spec (xv : ℤ) (yv : ℤ):
     simp [Example3.pay_index, Example3.lang_index, Example3.lang_fun_list, Example3.lang_squeeze_list,
       exists_labType, ← lang_sn1.eq_1]
     constructor
-    { rintro ⟨_, _⟩ ; subst al atrm
-      exists 1, trm_funs [trm_varl "xl", trm_varl "yl"] (lang_sn1 ap)
-      simp ; rw [(haux _ ap).mp rfl] ; rfl
+    { rintro ⟨_, _, _⟩ ; subst al atrm
+      exists 1, trm_funs [trm_varl "xl", trm_varl "yl"] (lang_sn1 (Int.toNat ap))
+      simp ; rw [(haux _ (Int.toNat ap)).mp rfl] ; simp ; assumption
     }
     { simp ; intros ; subst_eqs ; simp }
   }
@@ -384,8 +432,8 @@ lemma example4_spec (xv : ℤ) (yv : ℤ):
     constructor
     intro he1 he2 h1 h2 ; simp [hforall] at h1 h2
     rcases hin with (hin | hin)
-    · specialize h1 ip (by left ; simp [hin])
-      specialize h2 ip (by left ; simp [hin])
+    · specialize h1 (Int.toNat ip) (by left ; simp [hin])
+      specialize h2 (Int.toNat ip) (by left ; simp [hin])
       have tmp := HPropExact.isExact _ _ h1 h2 ; exact tmp
     · rcases hin with ⟨_, ⟨n, hin⟩, _⟩ ; subst_eqs ; simp at h1 h2
       specialize h1 n rfl ; specialize h2 n rfl
@@ -424,7 +472,7 @@ lemma example4_spec (xv : ℤ) (yv : ℤ):
   }
   { simp }
   { simp [forall_labType, exists_labType, lang_index, lang_squeeze_list', pay_index]
-    intro hv hh hpre a b c d ; specialize hpre _ a b c rfl d ; exact hpre
+    intro hv hh hpre a b c d ; specialize hpre _ a b c rfl d ; aesop
   }
 
 /- Previously, constraints for payloads in the heap are in the post-condition
